ulib/FStar.ReflexiveTransitiveClosure.fst
@@ -4,12 +4,20 @@ open FStar.Tactics
 
 #set-options "--max_ifuel 1 --max_fuel 0"
 
+noeq
+type _closure (#a:Type0) (r:relation a) : a -> a -> Type0 =
+| Refl: x:a -> _closure r x x
+| Step: x:a -> y:a -> r x y ->_closure r x y
+| Closure: x:a -> y:a -> z:a -> _closure r x y -> _closure r y z -> _closure r x z
+
+val closure_reflexive: #a:Type0 -> r:relation a -> Lemma (reflexive (_closure r))
 let closure_reflexive #a r =
-  assert (forall x. closure r x x) by
+  assert (forall x. _closure r x x) by
     (let x = forall_intro () in mapply (`Refl))
 
+val closure_transitive: #a:Type0 -> r:relation a -> Lemma (transitive (_closure r))
 let closure_transitive #a r =
-  assert (transitive (closure r)) by
+  assert (transitive (_closure r)) by
     (let x = forall_intro () in
      let y = forall_intro () in
      let z = forall_intro () in
@@ -18,11 +26,25 @@ let closure_transitive #a r =
      let _ = implies_intros () in
      seq (fun _ -> mapply (`Closure)) assumption)
 
-val _stable_on_closure: #a:Type0 -> r:relation a -> p:(a -> Type0) 
-  -> p_stable_on_r: squash (forall x y. p x /\ r x y ==> p y) 
-  -> x: a 
+let closure #a r =
+  closure_reflexive r;
+  closure_transitive r;
+  _closure r
+
+let closure_step #a r x y =
+  assert (r x y ==> closure r x y) by
+    (let xy = implies_intro () in
+     let xy : r x y = unquote (binder_to_term xy) in
+     squash_intro ();
+     exact (quote (Step #a #r x y xy)))
+
+let closure_inversion #a r x y = ()
+
+val _stable_on_closure: #a:Type0 -> r:relation a -> p:(a -> Type0)
+  -> p_stable_on_r: squash (forall x y. p x /\ r x y ==> p y)
+  -> x: a
   -> y: a
-  -> xy: closure r x y
+  -> xy: _closure r x y
   -> px: squash (p x)
   -> GTot (squash (p y)) (decreases xy)
 let rec _stable_on_closure #a r p p_stable_on_r x y xy px =
@@ -45,22 +67,4 @@ let stable_on_closure #a r p hr =
      let px = implies_intro () in
      let xy = implies_intro () in
      let xy : closure r x y = unquote (binder_to_term xy) in
-     exact (quote (_stable_on_closure r p hr x y xy (Squash.get_proof _))))     
-
-/// Test
-
-type state = | A | B | C 
-
-let r x y = 
-  match x, y with 
-  | A, B | B, C | C, B -> True
-  | _ -> False
-
-let p = function 
-  | A -> False 
-  | B | C -> True 
-
-let cl = reflexive_transitive_closure r
-
-let reachable_from_B (x:state{ cl B x }) : Lemma (x = B \/ x = C) =
-  stable_on_closure r p ()
+     exact (quote (_stable_on_closure r p hr x y xy (Squash.get_proof _))))
